using enumerated datatype

Dafny/cleanup3/Blood.dfy
@@ -1,13 +1,14 @@
 
+datatype BloodType = AP | BP | OP | ABP | AM | BM | OM | ABM
 
-predicate validBloodType(bloodType: string)
+predicate validBloodType(bloodType: BloodType)
 {
-    bloodType in ["A+", "B+", "O+", "AB+", "A-", "B-", "O-", "AB-"]
+    bloodType in [AP, BP, OP, ABP, AM, BM, OM, ABM]
 }
 
 class Blood
 {
-    var bloodType: string;
+    var bloodType: BloodType;
     var donorName: string;
     var dateDonated: int;
     var locationAcquired: string;
@@ -18,12 +19,12 @@ class Blood
         validBloodType(bloodType)
     }
 
-    constructor(bloodType: string,
-                donorName: string,
-                dateDonated: int,
+    constructor(bloodType:        BloodType,
+                donorName:        string,
+                dateDonated:      int,
                 locationAcquired: string)
         modifies this;
-        requires validBloodType(bloodType);
+        // requires validBloodType(bloodType);
         ensures  Valid();
         ensures  this.bloodType == bloodType;
         ensures  this.donorName == donorName;
@@ -36,7 +37,7 @@ class Blood
         this.locationAcquired := locationAcquired;
     }
 
-    function method GetBloodType(): string
+    function method GetBloodType(): BloodType
         reads this;
     {
         bloodType
@@ -79,30 +80,13 @@ class Blood
 
 method TestBlood()
 {
-    var bobsBlood := new Blood("A-", "Bob", 12, "Prince Wales Hospital");
+    var bobsBlood := new Blood(AM, "Bob", 12, "Prince Wales Hospital");
     
-    assert bobsBlood.GetBloodType() == "A-";
+    assert bobsBlood.GetBloodType() == AM;
     assert bobsBlood.GetDonorName() == "Bob";
     assert bobsBlood.GetDateDonated() == 12;
     bobsBlood.PrettyPrint();
 
-    // assert bobsBlood.GetBloodType() == "A-";
-    // assert bobsBlood.GetBloodType() != "A+";
-
-    // // Query
-    // var inv := new Blood[4];
-    // inv[0] := new Blood("B+", "Ava", 9);
-    // inv[1] := new Blood("A-", "Bob", 12);
-    // inv[2] := new Blood("O+", "Cal", 12);
-    // inv[3] := new Blood("AB+", "Deb", 13);
-    
-    // // (currently only seems to work with the last item in the inv)
-    // // maybe change bloodType to an enumeration?
-    // var r := queryBloodByType(inv, "AB+");
-    // assert r.Length == 1;
-    // assert r[0].GetDonorName() == "Deb";
-    
-    // assert countBloodByDate(inv, 10, 12) == 2;
-    // assert countBloodByType(inv, "AB+") == 1;
-    // print "\nQuery successful\n";
+    assert bobsBlood.GetBloodType() == AM;
+    assert bobsBlood.GetBloodType() != AP;
 }
